src/dafny/util/int.dfy
@@ -12,10 +12,12 @@
  * under the License.
  */
 
+include "../../../libs/DafnyCrypto/src/dafny/util/math.dfy"
 include "../../../libs/DafnyCrypto/src/dafny/util/option.dfy"
 
 module Int {
     import opened Optional
+    import MathUtils
 
     const TWO_7   : int := 0x0_80
     const TWO_8   : int := 0x1_00
@@ -123,104 +125,7 @@ module Int {
             case 20 => MAX_U160
             case 32 => MAX_U256
             // Fall back case (for now)
-            case _ => Pow(2,n) - 1
-    }
-
-    // =========================================================
-    // Exponent
-    // =========================================================
-
-    /**
-     * Compute n^k.
-     */
-    function Pow(n:nat, k:nat) : (r:nat)
-    // Following needed for some proofs
-    ensures n > 0 ==> r > 0 {
-        if k == 0 then 1
-        else if k == 1 then n
-        else
-            var p := k / 2;
-            var np := Pow(n,p);
-            if p*2 == k then np * np
-            else
-                np * np * n
-    }
-
-    // Simple lemma about POW.
-    lemma lemma_pow2(k:nat)
-    ensures Pow(2,k) > 0 {
-        if k == 0 {
-            assert Pow(2,k) == 1;
-        } else if k == 1 {
-            assert Pow(2,k) == 2;
-        } else {
-            lemma_pow2(k/2);
-        }
-    }
-
-    /**
-     * Compute n^k % m.  This is more efficient that doing Pow(n,k) % m.  In
-     * essence, this works by recursive decomposing the work and squaring the
-     * results.
-     */
-    function ModPow(n:nat, k:nat, m:nat) : (r:nat)
-    requires m > 0
-    ensures r < m
-    ensures n > 0 ==> r >= 0
-    decreases k {
-        var nm := n % m;
-        if k == 0 || m == 1 then 1%m
-        else if k == 1 then nm
-        else
-            var np := ModPow(nm,k/2,m);
-            var np2 := (np * np) % m;
-            if (k%2) == 0 then
-                // Even case.  n^2k = n^k * n^k
-                np2
-            else
-                // Odd case.  n^2k+1 = n^2k * n
-                (np2 * nm) % m
-    }
-
-    // Euclid's extended GCD algorithm, implemented recursively.
-    function GcdExtended(a: nat, b: nat) : (r:(nat,int,int))
-    // Conditions under which gcd is non-zero
-    ensures b > 0 ==> r.0 > 0
-    // Bezout's identity
-    ensures (a*r.1)+(b*r.2) == r.0 {
-        if a == 0 then (b,0,1)
-        else
-            var (g,x,y) := GcdExtended(b%a,a);
-            (g,y-((b/a)*x),x)
-    }
-
-    /// Determine multiplicative inverse of an element a under mod n.
-    function Inverse(a: nat, n: nat) : (r:Option<nat>)
-    requires a < n {
-        var (gcd,x,y) := GcdExtended(a,n);
-        if gcd > 1 then None
-        else if x >= 0 then Some(x)
-        else
-            // Following property is known to hold for Euclid's extended
-            // algorithm.  Unfortunately, I did not yet figure out how to get
-            // Dafny to prove this for us.
-            assume {:axiom} Abs(x) < n;
-            // Done
-            Some(x+n)
-    }
-
-    // A prime number is a natural greater than 1 that is divisible by any
-    // smaller number (except 1).
-    predicate IsPrime(n: nat) {
-        n > 1 && forall a :: 1 <= a < n ==> GcdExtended(a,n).0 == 1
-    }
-
-    // Every element in a prime field has a multiplicative inverse.
-    lemma PrimeFieldsHaveInverse(a:nat, n: nat)
-    requires IsPrime(n)
-    requires 1 <= a < n
-    ensures Inverse(a,n) != None {
-        assert GcdExtended(a,n).0 == 1;
+            case _ => MathUtils.Pow(2,n) - 1
     }
 
     // =========================================================
@@ -617,7 +522,7 @@ module U256 {
     {
         if rhs >= 256 then 0
         else
-            var p := Pow(2,rhs as nat);
+            var p := MathUtils.Pow(2,rhs as nat);
             var n := (lhs as nat) * p;
             (n % TWO_256) as u256
     }
@@ -625,7 +530,7 @@ module U256 {
     function Shr(lhs: u256, rhs: u256) : u256 {
         if rhs >= 256 then 0
         else
-            var p := Pow(2, rhs as nat);
+            var p := MathUtils.Pow(2, rhs as nat);
             var n := (lhs as nat) / p;
             n as u256
     }
@@ -773,7 +678,7 @@ module I256 {
         else if rhs < 256
         then
             assert 0 < rhs < 256;
-            var r := Pow(2,rhs as nat);
+            var r := MathUtils.Pow(2,rhs as nat);
             ((lhs as int) / (r as int)) as i256
         else if lhs < 0 then -1
         else 0
